memory_refine.v
@@ -43,7 +43,7 @@ Hint Extern 0 (_ ≤ length _) => solve_length.
 Hint Extern 0 (length _ ≤ _) => solve_length.
 
 Lemma mem_lookup_refine Γ α f Γm1 Γm2 m1 m2 a1 a2 v1 τ :
-  ✓ Γ → m1 ⊑{Γ,α,f@Γm1↦Γm2} m2 → a1 ⊑{Γ,α,f@Γm1↦Γm2} a2 : τ →
+  ✓ Γ → m1 ⊑{Γ,α,f@Γm1↦Γm2} m2 → a1 ⊑{Γ,α,f@Γm1↦Γm2} a2 : τ → τ ≠ voidT →
   m1 !!{Γ} a1 = Some v1 →
   ∃ v2, m2 !!{Γ} a2 = Some v2 ∧ v1 ⊑{Γ,α,f@Γm1↦Γm2} v2 : τ.
 Proof.
@@ -55,10 +55,10 @@ Proof.
     pbits_refine_kind_subseteq, ctree_flatten_refine; eauto using to_val_refine.
 Qed.
 Lemma mem_force_refine Γ α f Γm1 Γm2 m1 m2 a1 a2 τ :
-  ✓ Γ → m1 ⊑{Γ,α,f@Γm1↦Γm2} m2 → a1 ⊑{Γ,α,f@Γm1↦Γm2} a2 : τ →
+  ✓ Γ → m1 ⊑{Γ,α,f@Γm1↦Γm2} m2 → a1 ⊑{Γ,α,f@Γm1↦Γm2} a2 : τ → τ ≠ voidT →
   is_Some (m1 !!{Γ} a1) → mem_force Γ a1 m1 ⊑{Γ,α,f@Γm1↦Γm2} mem_force Γ a2 m2.
 Proof.
-  unfold lookupE, mem_lookup, mem_force. intros ??? [v1 ?].
+  unfold lookupE, mem_lookup, mem_force. intros ???? [v1 ?].
   destruct (m1 !!{Γ} a1) as [w1|] eqn:?; simplify_option_equality.
   destruct (cmap_lookup_refine Γ α f Γm1 Γm2
     m1 m2 a1 a2 w1 τ) as (w2&?&?); auto.
@@ -66,29 +66,29 @@ Proof.
     pbits_refine_kind_subseteq, ctree_flatten_refine.
 Qed.
 Lemma mem_force_refine' Γ α f m1 m2 a1 a2 τ :
-  ✓ Γ → m1 ⊑{Γ,α,f} m2 → a1 ⊑{Γ,α,f@'{m1}↦'{m2}} a2 : τ →
+  ✓ Γ → m1 ⊑{Γ,α,f} m2 → a1 ⊑{Γ,α,f@'{m1}↦'{m2}} a2 : τ → τ ≠ voidT →
   is_Some (m1 !!{Γ} a1) → mem_force Γ a1 m1 ⊑{Γ,α,f} mem_force Γ a2 m2.
 Proof.
-  unfold refineM, cmap_refine'; intros ??? [v1 ?].
+  unfold refineM, cmap_refine'; intros ???? [v1 ?].
   destruct (mem_lookup_refine Γ α f ('{m1}) ('{m2})
     m1 m2 a1 a2 v1 τ) as (v2&?&?); eauto.
   erewrite !mem_force_memenv_of by eauto using cmap_refine_valid_l',
     cmap_refine_valid_r'; eauto using mem_force_refine.
 Qed.
 Lemma mem_writable_refine Γ α f Γm1 Γm2 m1 m2 a1 a2 τ :
-  ✓ Γ → m1 ⊑{Γ,α,f@Γm1↦Γm2} m2 → a1 ⊑{Γ,α,f@Γm1↦Γm2} a2 : τ →
+  ✓ Γ → m1 ⊑{Γ,α,f@Γm1↦Γm2} m2 → a1 ⊑{Γ,α,f@Γm1↦Γm2} a2 : τ → τ ≠ voidT →
   mem_writable Γ a1 m1 → mem_writable Γ a2 m2.
 Proof.
-  intros ??? (w1&?&?). destruct (cmap_lookup_refine Γ α f Γm1 Γm2
+  intros ???? (w1&?&?). destruct (cmap_lookup_refine Γ α f Γm1 Γm2
     m1 m2 a1 a2 w1 τ) as (w2&?&?); auto.
   exists w2; eauto using pbits_refine_kind_subseteq, ctree_flatten_refine.
 Qed.
 Lemma mem_insert_refine Γ α f Γm1 Γm2 m1 m2 a1 a2 v1 v2 τ :
-  ✓ Γ → m1 ⊑{Γ,α,f@Γm1↦Γm2} m2 → a1 ⊑{Γ,α,f@Γm1↦Γm2} a2 : τ →
+  ✓ Γ → m1 ⊑{Γ,α,f@Γm1↦Γm2} m2 → a1 ⊑{Γ,α,f@Γm1↦Γm2} a2 : τ → τ ≠ voidT →
   mem_writable Γ a1 m1 → v1 ⊑{Γ,α,f@Γm1↦Γm2} v2 : τ →
   <[a1:=v1]{Γ}>m1 ⊑{Γ,α,f@Γm1↦Γm2} <[a2:=v2]{Γ}>m2.
 Proof.
-  intros ??? (w1&?&?) ?. destruct (cmap_lookup_refine Γ α f Γm1 Γm2
+  intros ???? (w1&?&?) ?. destruct (cmap_lookup_refine Γ α f Γm1 Γm2
     m1 m2 a1 a2 w1 τ) as (w2&?&?); auto.
   eapply cmap_alter_refine; eauto 1.
   * eapply ctree_Forall_not, pbits_mapped; eauto using pbits_kind_weaken.
@@ -104,7 +104,7 @@ Proof.
 Qed.
 Lemma mem_insert_refine' Γ α f m1 m2 a1 a2 v1 v2 τ :
   ✓ Γ → m1 ⊑{Γ,α,f} m2 →
-  a1 ⊑{Γ,α,f@'{m1}↦'{m2}} a2 : τ → mem_writable Γ a1 m1 →
+  a1 ⊑{Γ,α,f@'{m1}↦'{m2}} a2 : τ → τ ≠ voidT → mem_writable Γ a1 m1 →
   v1 ⊑{Γ,α,f@'{m1}↦'{m2}} v2 : τ → <[a1:=v1]{Γ}>m1 ⊑{Γ,α,f} <[a2:=v2]{Γ}>m2.
 Proof.
   unfold refineM, cmap_refine'; intros.
@@ -245,7 +245,7 @@ Proof.
 Qed.
 Lemma mem_alloc_val_refine' Γ α f m1 m2 malloc o1 o2 v1 v2 τ :
   ✓ Γ → m1 ⊑{Γ,α,f} m2 → v1 ⊑{Γ,α,f@'{m1}↦'{m2}} v2 : τ →
-  int_typed (size_of Γ τ) sptrT →
+  τ ≠ voidT → int_typed (size_of Γ τ) sptrT →
   mem_allocable o1 m1 → mem_allocable o2 m2 → ∃ f',
   (**i 1.) *) f' !! o1 = Some (o2,[]) ∧
   (**i 2.) *) <[addr_top o1 τ:=v1]{Γ}>(mem_alloc Γ o1 malloc τ m1)
@@ -264,14 +264,15 @@ Hint Immediate cmap_refine_memenv_refine.
 Lemma mem_alloc_val_list_refine' Γ α f m1 m2 os1 os2 vs1 vs2 τs :
   ✓ Γ → m1 ⊑{Γ,α,f} m2 → vs1 ⊑{Γ,α,f@'{m1}↦'{m2}}* vs2 :* τs →
   length os1 = length vs1 → length os2 = length vs2 →
-  Forall (λ τ, int_typed (size_of Γ τ) sptrT) τs →
+  Forall (λ τ, int_typed (size_of Γ τ) sptrT) τs → Forall (≠ voidT) τs →
   mem_allocable_list m1 os1 → mem_allocable_list m2 os2 → ∃ f',
   (**i 1.) *) Forall2 (λ o1 o2, f' !! o1 = Some (o2,[])) os1 os2 ∧
   (**i 2.) *) mem_alloc_val_list Γ (zip os1 vs1) m1
       ⊑{Γ,α,f'} mem_alloc_val_list Γ (zip os2 vs2) m2 ∧
   (**i 3.) *) meminj_extend f f' ('{m1}) ('{m2}).
 Proof.
-  rewrite <-!Forall2_same_length. intros ? Hm Hvs Hovs1 Hovs2 Hτs Hos1 Hos2.
+  rewrite <-!Forall2_same_length.
+  intros ? Hm Hvs Hovs1 Hovs2 Hτs Hvoids Hos1 Hos2.
   revert f os1 os2 vs1 vs2 m1 m2 Hm Hos1 Hos2 Hvs Hovs1 Hovs2.
   induction Hτs as [|τ τs ?? IH];
     intros f ?? vs1' vs2' m1 m2 ? [|o1 os1 ???] [|o2 os2 ???];
@@ -282,7 +283,7 @@ Proof.
   assert (✓{Γ} τ) by eauto using val_typed_type_valid.
   destruct (mem_alloc_val_refine' Γ α f m1 m2 false o1 o2 v1 v2 τ)
     as (f'&?&?&?); auto; simplify_type_equality.
-  edestruct (IH f' os1 os2 vs1 vs2) as (f''&?&?&?); eauto.
+  edestruct (λ H, IH H f' os1 os2 vs1 vs2) as (f''&?&?&?); eauto.
   { rewrite mem_insert_allocable_list; eauto using mem_alloc_allocable_list. }
   { rewrite mem_insert_allocable_list; eauto using mem_alloc_allocable_list. }
   { eauto using vals_refine_weaken, mem_alloc_val_forward. }
@@ -501,10 +502,10 @@ Proof.
   by rewrite pbits_locked_mask, fmap_take, fmap_drop, lookup_take, lookup_drop.
 Qed.
 Lemma mem_lock_refine Γ α f Γm1 Γm2 m1 m2 a1 a2 τ : 
-  ✓ Γ → m1 ⊑{Γ,α,f@Γm1↦Γm2} m2 → a1 ⊑{Γ,α,f@Γm1↦Γm2} a2 : τ →
+  ✓ Γ → m1 ⊑{Γ,α,f@Γm1↦Γm2} m2 → a1 ⊑{Γ,α,f@Γm1↦Γm2} a2 : τ → τ ≠ voidT →
   mem_writable Γ a1 m1 → mem_lock Γ a1 m1 ⊑{Γ,α,f@Γm1↦Γm2} mem_lock Γ a2 m2.
 Proof.
-  intros ??? (w1&?&?). assert (∀ xb, pbit_indetify xb = xb →
+  intros ???? (w1&?&?). assert (∀ xb, pbit_indetify xb = xb →
     pbit_indetify (pbit_lock xb) = pbit_lock xb) by (by intros ? <-).
   destruct (cmap_lookup_refine Γ α f Γm1 Γm2 m1 m2 a1 a2 w1 τ) as (w2&?&?); auto.
   eapply cmap_alter_refine; eauto 1.
@@ -516,7 +517,7 @@ Proof.
     eauto using pbits_lock_mapped, pbits_mapped, pbits_kind_weaken.
 Qed.
 Lemma mem_lock_refine' Γ α f m1 m2 a1 a2 τ : 
-  ✓ Γ → m1 ⊑{Γ,α,f} m2 → a1 ⊑{Γ,α,f@'{m1}↦'{m2}} a2 : τ →
+  ✓ Γ → m1 ⊑{Γ,α,f} m2 → a1 ⊑{Γ,α,f@'{m1}↦'{m2}} a2 : τ → τ ≠ voidT →
   mem_writable Γ a1 m1 → mem_lock Γ a1 m1 ⊑{Γ,α,f} mem_lock Γ a2 m2.
 Proof.
   intros. unfold refineM, cmap_refine'. erewrite !mem_lock_memenv_of by eauto
@@ -533,7 +534,7 @@ Proof.
   revert w1 w2 τ Hw βs Hlen.
   refine (ctree_refine_ind _ _ _ _ _ _ _ _ _ _ _ _); simpl.
   * constructor; auto using pbits_unlock_refine.
-  * intros τ n ws1 ws2 -> ? IH _ βs. rewrite bit_size_of_array. intros Hlen.
+  * intros τ n ws1 ws2 -> ? IH ? _ βs. rewrite bit_size_of_array. intros Hlen.
     constructor. revert βs Hlen. induction IH; intros; decompose_Forall_hyps;
       erewrite ?Forall2_length by eauto using ctree_flatten_refine; auto.
   * intros s τs wxbss1 wxbss2 Hs Hws IH Hxbss _ _ Hpad βs.
